Use Mathlib to prove that sqrt(2) is irrational.

Strata/DL/Util/List.lean
@@ -22,21 +22,21 @@ theorem List.subset_append_cons_right {α : Type} [DecidableEq α] {a b c : List
 /--
 Remove duplicates in a list.
 -/
-def dedup {α : Type} [DecidableEq α] : List α → List α
+def deduplicate {α : Type} [DecidableEq α] : List α → List α
   | [] => []
   | a :: as =>
-    let as := as.dedup
+    let as := as.deduplicate
     if a ∈ as then as else a :: as
 
 /--
 A deduplicated list satisfies `Nodup`.
 -/
-theorem nodup_dedup {α : Type} [DecidableEq α] (l : List α) :
-  l.dedup.Nodup := by
+theorem nodup_deduplicate {α : Type} [DecidableEq α] (l : List α) :
+  l.deduplicate.Nodup := by
   induction l with
-  | nil => simp [dedup]
+  | nil => simp [deduplicate]
   | cons a as ih =>
-    simp [dedup]
+    simp [deduplicate]
     split
     · exact ih
     · rename_i h; constructor
@@ -48,11 +48,11 @@ The upper bound of the length of a deduplicated list is the length of the
 original list.
 -/
 theorem length_dedup_le {α : Type} [DecidableEq α] (l : List α) :
-  l.dedup.length ≤ l.length := by
+  l.deduplicate.length ≤ l.length := by
   induction l with
-  | nil => simp [dedup]
+  | nil => simp [deduplicate]
   | cons a as ih =>
-    simp [dedup]
+    simp [deduplicate]
     split
     · exact Nat.le_succ_of_le ih
     · simp; exact ih
@@ -62,25 +62,25 @@ The lower bound of the length of a deduplicated list with an element consed onto
 it (i.e., `(a :: l)`) is the length of the deduplicated list `l`.
 -/
 theorem length_dedup_cons_le {α : Type} [DecidableEq α] (a : α) (l : List α) :
-  l.dedup.length ≤ (a :: l).dedup.length := by
+  l.deduplicate.length ≤ (a :: l).deduplicate.length := by
   induction l with
-  | nil => simp [dedup]
+  | nil => simp [deduplicate]
   | cons a as ih =>
-    simp [dedup]
+    simp [deduplicate]
     split
     · exact ih
     · rename_i a' h
       simp_all
       by_cases a' = a
       · simp_all
-      · by_cases a' ∈ as.dedup <;> simp_all
+      · by_cases a' ∈ as.deduplicate <;> simp_all
 
 theorem mem_dedup_of_mem {α : Type} [DecidableEq α]
-  (l : List α) (a : α) : a ∈ l.dedup → a ∈ l := by
+  (l : List α) (a : α) : a ∈ l.deduplicate → a ∈ l := by
   induction l with
-  | nil => simp [dedup]
+  | nil => simp [deduplicate]
   | cons b bs ih =>
-    simp [dedup]
+    simp [deduplicate]
     split
     · intro h
       exact Or.symm (Or.intro_left (a = b) (ih h))
@@ -89,39 +89,39 @@ theorem mem_dedup_of_mem {α : Type} [DecidableEq α]
       | head => exact Or.symm (Or.inr rfl)
       | tail _ h' => exact Or.symm (Or.intro_left (a = b) (ih h'))
 
-theorem mem_of_mem_dedup {α : Type} [DecidableEq α]
-  (l : List α) (a : α) : a ∈ l → a ∈ l.dedup := by
+theorem mem_of_mem_deduplicate {α : Type} [DecidableEq α]
+  (l : List α) (a : α) : a ∈ l → a ∈ l.deduplicate := by
   induction l with
-  | nil => simp [dedup]
+  | nil => simp [deduplicate]
   | cons b bs ih =>
-    simp [dedup]
+    simp [deduplicate]
     intro h; cases h
     · subst a
-      by_cases b ∈ bs.dedup <;> simp_all
-    · by_cases b ∈ bs.dedup <;> simp_all
+      by_cases b ∈ bs.deduplicate <;> simp_all
+    · by_cases b ∈ bs.deduplicate <;> simp_all
 
 /--
 An element `a` is in a list `l` iff it is in the deduplicated version
 of `l`.
 -/
-theorem mem_of_dedup {α : Type} [DecidableEq α]
-  (l : List α) (a : α) : a ∈ l ↔ a ∈ l.dedup := by
+theorem mem_of_deduplicate {α : Type} [DecidableEq α]
+  (l : List α) (a : α) : a ∈ l ↔ a ∈ l.deduplicate := by
   apply Iff.intro
-  exact fun h => mem_of_mem_dedup l a h
+  exact fun h => mem_of_mem_deduplicate l a h
   exact fun h => mem_dedup_of_mem l a h
 
 theorem length_dedup_cons_of_mem {α : Type} [DecidableEq α] (a : α) (l : List α)
-  (h : a ∈ l) : (a :: l).dedup.length = l.dedup.length := by
-  simp [dedup]
-  have : a ∈ l.dedup := mem_of_mem_dedup l a h
+  (h : a ∈ l) : (a :: l).deduplicate.length = l.deduplicate.length := by
+  simp [deduplicate]
+  have : a ∈ l.deduplicate := mem_of_mem_deduplicate l a h
   simp [this]
 
 theorem length_dedup_cons_of_not_mem {α : Type} [DecidableEq α] (a : α) (l : List α)
-  (h : a ∉ l) : (a :: l).dedup.length = 1 + l.dedup.length := by
+  (h : a ∉ l) : (a :: l).deduplicate.length = 1 + l.deduplicate.length := by
   induction l
-  · simp_all [dedup]
+  · simp_all [deduplicate]
   · rename_i head tail ih
-    simp_all [dedup]
+    simp_all [deduplicate]
     obtain ⟨h1, h2⟩ := h
     split
     · have := @mem_dedup_of_mem _ _ tail a
@@ -131,53 +131,53 @@ theorem length_dedup_cons_of_not_mem {α : Type} [DecidableEq α] (a : α) (l : 
       simp_all
       omega
 
-theorem mem_append_left_of_mem_dedup {α : Type} [DecidableEq α] (a : α) (l₁ l₂ : List α)
-  (h1 : ¬a ∈ l₂.dedup) (h2 : a ∈ (l₁ ++ l₂).dedup) :
+theorem mem_append_left_of_mem_deduplicate {α : Type} [DecidableEq α] (a : α) (l₁ l₂ : List α)
+  (h1 : ¬a ∈ l₂.deduplicate) (h2 : a ∈ (l₁ ++ l₂).deduplicate) :
   a ∈ l₁ := by
   have := @mem_dedup_of_mem _ _ (l₁ ++ l₂) a (by assumption)
   have := @mem_dedup_of_mem _ _ l₂ a
   simp_all; cases this
   · assumption
-  · have := @mem_of_mem_dedup _ _ l₂ a (by assumption)
+  · have := @mem_of_mem_deduplicate _ _ l₂ a (by assumption)
     contradiction
 
-theorem mem_append_right_of_mem_dedup {α : Type} [DecidableEq α] (a : α) (l₁ l₂ : List α)
-  (h1 : ¬a ∈ l₁.dedup) (h2 : a ∈ (l₁ ++ l₂).dedup) :
+theorem mem_append_right_of_mem_deduplicate {α : Type} [DecidableEq α] (a : α) (l₁ l₂ : List α)
+  (h1 : ¬a ∈ l₁.deduplicate) (h2 : a ∈ (l₁ ++ l₂).deduplicate) :
   a ∈ l₂ := by
   have := @mem_dedup_of_mem _ _ (l₁ ++ l₂) a (by assumption)
   have := @mem_dedup_of_mem _ _ l₁ a
   simp_all; cases this
-  · have := @mem_of_mem_dedup _ _ l₁ a (by assumption)
+  · have := @mem_of_mem_deduplicate _ _ l₁ a (by assumption)
     contradiction
   · assumption
 
 theorem length_dedup_append_le_sum {α : Type} [DecidableEq α] (l₁ l₂ : List α) :
-  (l₁ ++ l₂).dedup.length ≤ l₁.dedup.length + l₂.dedup.length := by
+  (l₁ ++ l₂).deduplicate.length ≤ l₁.deduplicate.length + l₂.deduplicate.length := by
   induction l₁ generalizing l₂
   · simp_all
   · rename_i head tail ih
-    simp [dedup]
-    by_cases h1 : head ∈ tail.dedup
-    · have : head ∈ (tail ++ l₂).dedup := by
+    simp [deduplicate]
+    by_cases h1 : head ∈ tail.deduplicate
+    · have : head ∈ (tail ++ l₂).deduplicate := by
         have := @mem_dedup_of_mem _ _ tail head h1
-        have := @mem_of_mem_dedup _ _ (tail ++ l₂) head
+        have := @mem_of_mem_deduplicate _ _ (tail ++ l₂) head
         simp_all
       simp_all
     · simp_all
-      by_cases h2 : head ∈ l₂.dedup
-      · have : head ∈ (tail ++ l₂).dedup := by
+      by_cases h2 : head ∈ l₂.deduplicate
+      · have : head ∈ (tail ++ l₂).deduplicate := by
           have := @mem_dedup_of_mem _ _ l₂ head  h2
-          have := @mem_of_mem_dedup _ _ (tail ++ l₂) head
+          have := @mem_of_mem_deduplicate _ _ (tail ++ l₂) head
           simp_all
         simp_all
         have := ih l₂
         omega
-      · have : head ∉ (tail ++ l₂).dedup := by
+      · have : head ∉ (tail ++ l₂).deduplicate := by
           have := @mem_dedup_of_mem _ _ (tail ++ l₂) head
           intro h
           simp_all
-          have := @mem_of_mem_dedup _ _ tail head
-          have := @mem_of_mem_dedup _ _ l₂ head
+          have := @mem_of_mem_deduplicate _ _ tail head
+          have := @mem_of_mem_deduplicate _ _ l₂ head
           simp_all
         simp_all
         have := ih l₂
@@ -193,23 +193,23 @@ theorem removeAll_of_cons {α : Type} [DecidableEq α] (x : α) (xs ys : List α
 
 theorem length_dedup_of_removeAll {α : Type} [DecidableEq α] (a : α) (l : List α)
   (h : a ∈ l) :
-  l.dedup.length = 1 + (l.removeAll [a]).dedup.length := by
+  l.deduplicate.length = 1 + (l.removeAll [a]).deduplicate.length := by
   induction l
   case nil => simp_all
   case cons x xs ih =>
-    simp [dedup]
+    simp [deduplicate]
     simp at h
     by_cases h : a = x
     case pos =>
       subst a
       split
       · rename_i h_x_xs
-        have : x ∈ xs := by exact (mem_of_dedup xs x).mpr h_x_xs
+        have : x ∈ xs := by exact (mem_of_deduplicate xs x).mpr h_x_xs
         have ih' := ih this
         simp_all [removeAll]
       · simp [removeAll]
         have : x ∉ xs := by
-          have := @mem_of_dedup _ _ xs x
+          have := @mem_of_deduplicate _ _ xs x
           simp_all
         have : (filter (fun x_1 => !decide (x_1 = x)) xs) = xs := by
           simp_all
@@ -229,7 +229,7 @@ theorem length_dedup_of_removeAll {α : Type} [DecidableEq α] (a : α) (l : Lis
         have := @length_dedup_cons_of_mem _ _ x (xs.removeAll [a])
         have : x ∈ xs.removeAll [a] := by
           simp [removeAll, h']
-          exact (mem_of_dedup xs x).mpr hx
+          exact (mem_of_deduplicate xs x).mpr hx
         simp_all
       · rename_i h_x_not_in_xs
         simp_all
@@ -241,39 +241,39 @@ theorem length_dedup_of_removeAll {α : Type} [DecidableEq α] (a : α) (l : Lis
         have : ¬ x ∈ xs.removeAll [a] := by
           simp [removeAll]
           have : x ∉ xs := by
-            have := @mem_of_dedup _ _ xs x
+            have := @mem_of_deduplicate _ _ xs x
             simp_all
           simp_all
         simp_all
         omega
 
 theorem length_dedup_append_le_left {α : Type} [DecidableEq α] (l₁ l₂ : List α) :
-  l₁.dedup.length ≤ (l₁ ++ l₂).dedup.length := by
+  l₁.deduplicate.length ≤ (l₁ ++ l₂).deduplicate.length := by
   induction l₁ generalizing l₂
-  case nil => simp [dedup]
+  case nil => simp [deduplicate]
   case cons a as ih =>
-    simp [dedup]
+    simp [deduplicate]
     split
     · rename_i h
-      have : a ∈ as := by exact (mem_of_dedup as a).mpr h
-      have : a ∈ (as ++ l₂).dedup := by
+      have : a ∈ as := by exact (mem_of_deduplicate as a).mpr h
+      have : a ∈ (as ++ l₂).deduplicate := by
         have : a ∈ as ++ l₂ := by simp_all
-        exact (mem_of_dedup (as ++ l₂) a).mp this
+        exact (mem_of_deduplicate (as ++ l₂) a).mp this
       simp_all
-    · by_cases ha : a ∈ (as ++ l₂).dedup
+    · by_cases ha : a ∈ (as ++ l₂).deduplicate
       case pos =>
         rename_i h_a_as
         simp_all
         have h_l2 : ∃ l, l = l₂.removeAll [a] := by simp_all
         obtain ⟨l, hl⟩ := h_l2
         simp_all
-        have h_a_as_l2 : a ∈ as ++ l₂ := by exact (mem_of_dedup (as ++ l₂) a).mpr ha
+        have h_a_as_l2 : a ∈ as ++ l₂ := by exact (mem_of_deduplicate (as ++ l₂) a).mpr ha
         have h := @length_dedup_of_removeAll _ _ a (as ++ l₂) h_a_as_l2
         rw [h]
         have : ((as ++ l₂).removeAll [a]) = as ++ l := by
           simp [removeAll]
           have h_not_in_a_as : a ∉ as := by
-            have := @mem_of_dedup _ _ as a
+            have := @mem_of_deduplicate _ _ as a
             simp_all
           have h_a_as : filter (fun x => !decide (x = a)) as = as := by
             simp_all
@@ -290,7 +290,7 @@ theorem length_dedup_append_le_left {α : Type} [DecidableEq α] (l₁ l₂ : Li
 
 theorem length_dedup_append_all_in_right {α : Type} [DecidableEq α] (l₁ l₂ : List α)
   (h : l₁.all (fun e => e ∈ l₂)) :
-  (l₁ ++ l₂).dedup.length = l₂.dedup.length := by
+  (l₁ ++ l₂).deduplicate.length = l₂.deduplicate.length := by
   induction l₁
   · simp_all
   · rename_i head tail ih
@@ -300,22 +300,22 @@ theorem length_dedup_append_all_in_right {α : Type} [DecidableEq α] (l₁ l₂
     simp [@length_dedup_cons_of_mem _ _ head (tail ++ l₂) h1']
     induction tail <;> try simp
     rename_i x xrest ih
-    simp_all [dedup]
+    simp_all [deduplicate]
     have : x ∈ (xrest ++ l₂) := by simp_all
-    have : x ∈ (xrest ++ l₂).dedup := by
-      exact @mem_of_mem_dedup _ _ (xrest ++ l₂) x (by assumption)
+    have : x ∈ (xrest ++ l₂).deduplicate := by
+      exact @mem_of_mem_deduplicate _ _ (xrest ++ l₂) x (by assumption)
     simp_all
     done
 
 theorem length_dedup_append_subset_right {α : Type} [DecidableEq α] (l₁ l₂ : List α)
   (h : l₁ ⊆ l₂) :
-  (l₁ ++ l₂).dedup.length = l₂.dedup.length := by
+  (l₁ ++ l₂).deduplicate.length = l₂.deduplicate.length := by
   simp_all [List.instHasSubset, List.Subset]
   exact @length_dedup_append_all_in_right _ _ l₁ l₂ (by simp_all)
 
 theorem length_dedup_append_all_in_left {α : Type} [DecidableEq α] (l₁ l₂ : List α)
   (h : l₂.all (fun e => e ∈ l₁)) :
-  (l₁ ++ l₂).dedup.length = l₁.dedup.length := by
+  (l₁ ++ l₂).deduplicate.length = l₁.deduplicate.length := by
   induction l₂ generalizing l₁
   case nil => simp_all
   case cons x xs ih =>
@@ -333,36 +333,36 @@ theorem length_dedup_append_all_in_left {α : Type} [DecidableEq α] (l₁ l₂ 
 theorem length_dedup_all_in_eq {α : Type} [DecidableEq α] (l₁ l₂ : List α)
   (h1 : l₁.all (fun e => e ∈ l₂))
   (h2 : l₂.all (fun e => e ∈ l₁)) :
-  l₁.dedup.length = l₂.dedup.length := by
+  l₁.deduplicate.length = l₂.deduplicate.length := by
   have h_1 := @length_dedup_append_all_in_right _ _ l₁ l₂ h1
   have h_2 := @length_dedup_append_all_in_left _ _ l₁ l₂ h2
   simp_all
 
 theorem length_dedup_subset_eq {α : Type} [DecidableEq α] (l₁ l₂ : List α)
   (h1 : l₁ ⊆ l₂) (h2 : l₂ ⊆ l₁) :
-  l₁.dedup.length = l₂.dedup.length := by
+  l₁.deduplicate.length = l₂.deduplicate.length := by
   have := @length_dedup_all_in_eq _ _ l₁ l₂
   simp_all [List.instHasSubset, List.Subset]
 
 theorem length_dedup_append_le_right {α : Type} [DecidableEq α] (l₁ l₂ : List α) :
-  l₂.dedup.length ≤ (l₁ ++ l₂).dedup.length := by
+  l₂.deduplicate.length ≤ (l₁ ++ l₂).deduplicate.length := by
   have h_left := @length_dedup_append_le_left _ _ l₂ l₁
   have := @length_dedup_all_in_eq _ _ (l₁ ++ l₂) (l₂ ++ l₁)
   simp_all
 
 theorem length_dedup_of_all_in_not_mem_lt {α : Type} [DecidableEq α] (l₁ l₂ : List α) (a : α)
   (h1 : l₁.all (fun e => e ∈ l₂)) (h2 : a ∉ l₁) (h3 : a ∈ l₂) :
-  l₁.dedup.length < l₂.dedup.length := by
+  l₁.deduplicate.length < l₂.deduplicate.length := by
   induction l₁ generalizing l₂ with
   | nil =>
-    simp_all [dedup]
-    have : a ∈ l₂.dedup := by
-      have := @mem_of_dedup _ _ l₂ a
+    simp_all [deduplicate]
+    have : a ∈ l₂.deduplicate := by
+      have := @mem_of_deduplicate _ _ l₂ a
       simp_all
     exact length_pos_of_mem this
   | cons head tail ih =>
     simp at h1 ih
-    simp [dedup]
+    simp [deduplicate]
     obtain ⟨h1_head_l2, h1⟩ := h1
     split
     · rename_i h_head_tail
@@ -371,7 +371,7 @@ theorem length_dedup_of_all_in_not_mem_lt {α : Type} [DecidableEq α] (l₁ l�
       have h_head_tail := @length_dedup_cons_of_not_mem _ _ head tail
       by_cases h_head_in_tail : head ∈ tail
       case pos =>
-        simp_all [@mem_of_dedup _ _ tail head]
+        simp_all [@mem_of_deduplicate _ _ tail head]
       case neg =>
         have h_removeAll := @length_dedup_of_removeAll _ _ head l₂ h1_head_l2
         simp_all
@@ -389,14 +389,14 @@ theorem length_dedup_of_all_in_not_mem_lt {α : Type} [DecidableEq α] (l₁ l�
 
 theorem length_dedup_of_subset_not_mem_lt {α : Type} [DecidableEq α] (l₁ l₂ : List α) (a : α)
   (h1 : l₁ ⊆ l₂) (h2 : a ∉ l₁) (h3 : a ∈ l₂) :
-  l₁.dedup.length < l₂.dedup.length := by
+  l₁.deduplicate.length < l₂.deduplicate.length := by
   have := @length_dedup_of_all_in_not_mem_lt _ _ l₁ l₂ a
   simp_all [List.instHasSubset, List.Subset]
 
 theorem length_dedup_of_subset_le {α : Type} [DecidableEq α] (l₁ l₂ : List α)
-  (h : l₁ ⊆ l₂) : l₁.dedup.length ≤ l₂.dedup.length := by
+  (h : l₁ ⊆ l₂) : l₁.deduplicate.length ≤ l₂.deduplicate.length := by
   induction l₁ with
-  | nil => simp_all [dedup]
+  | nil => simp_all [deduplicate]
   | cons head tail ih =>
     have h_tail_l2 : tail ⊆ l₂ := by simp_all
     have ih' := @ih h_tail_l2
@@ -407,10 +407,10 @@ theorem length_dedup_of_subset_le {α : Type} [DecidableEq α] (l₁ l₂ : List
     case neg =>
       simp_all
       have := @length_dedup_of_subset_not_mem_lt _ _ tail l₂ head h_tail_l2 h_head h
-      have h_head_dedup : head ∉ tail.dedup := by
-        have := @mem_of_dedup _ _ tail head
+      have h_head_deduplicate : head ∉ tail.deduplicate := by
+        have := @mem_of_deduplicate _ _ tail head
         simp_all
-      simp_all [dedup]
+      simp_all [deduplicate]
       omega
 
 end List
