Strata/Languages/Boogie/Examples/IrratSqrt2.lean
@@ -1,0 +1,59 @@
+/-
+  Copyright Strata Contributors
+
+  SPDX-License-Identifier: Apache-2.0 OR MIT
+-/
+
+import Strata.Languages.Boogie.Boogie
+import Strata.Languages.Boogie.Verifier
+import Mathlib.Data.Real.Irrational
+
+---------------------------------------------------------------------
+namespace Strata
+
+def sqrt2IrrationalEnv : Environment :=
+#strata
+program Boogie;
+procedure Test(p : int, q : int) returns ()
+{
+  assume [q_gt_0]: (q > 0);
+  assert [sqrt_2_is_irrational]: ((p * p) != (2 * q * q));
+};
+#end
+
+private theorem sqrt_2_is_irrational_helper :
+  ∀ (p q : Int), (decide (q > 0) ==> !p * p == 2 * q * q) = true := by
+  intro p q
+  simp [Lambda.Bool.implies, -decide_implies]
+  intro h_q_pos
+  have h_main := irrational_sqrt_two
+  have h_not_isSq := @irrational_sqrt_ratCast_iff_of_nonneg 2 (by simp)
+  simp_all [IsSquare]
+  have h_not_isSq_alt := @h_not_isSq (p / q)
+  ring_nf at h_not_isSq_alt
+  have := @mul_inv_eq_iff_eq_mul₀  _ _
+          ((p : Rat) ^ 2) ((q : Rat) ^ 2) 2 (by simp_all; omega)
+  ring_nf at this
+  norm_cast at this
+  ring_nf; simp_all
+  have _ : ¬((p : Rat) ^ 2 * ((q : Rat) ^ 2)⁻¹ = 2) := by
+    exact fun a => h_not_isSq_alt (id (Eq.symm a))
+  simp_all
+
+
+theorem sqrt_2_is_irrational : ∀ («$__p0» «$__q1» : ℤ), (decide («$__q1» > 0) ==> !«$__p0» * «$__p0» == 2 * «$__q1» * «$__q1») = true := by
+  exact fun «$__p0» «$__q1» => sqrt_2_is_irrational_helper «$__p0» «$__q1»
+
+/--
+info: SMT Results:
+
+Obligation: sqrt_2_is_irrational
+Result: err ⏎
+---
+info:
+✅️ Theorem sqrt_2_is_irrational is already in the environment!
+-/
+#guard_msgs in
+#verify "cvc5" sqrt2IrrationalEnv
+
+end Strata
